MirrorCharge!/src/MirrorCharge/Java/MethodSpecTactics.v
@@ -66,7 +66,7 @@ Fixpoint search_NoDup
 
 Definition list_notin_set lst s :=
   	fold_right (fun a acc => andb (SS.for_all (fun b => negb (string_dec a b)) s) acc) true lst.
-
+(*
 Definition method_specI : stac typ (expr typ func) subst :=
   fun tus tvs s lst e =>
     match e with
@@ -100,7 +100,7 @@ Definition method_specI : stac typ (expr typ func) subst :=
     	      end
       	| _ => @Fail _ _ _
     end.
-
+*)
 
 Fixpoint get_alls (e : expr typ func) : list typ * expr typ func :=
   match e with
@@ -127,6 +127,18 @@ Definition convert_to_lemma (e : expr typ func)
    ; premises := impls
    ; concl := e |}.
 
+Ltac reify_lemma_aux T :=
+(let k e :=
+           let e := constr:(convert_to_lemma e) in
+           let e := eval unfold convert_to_lemma in e in
+           let e := eval simpl in e in
+           refine e
+       in
+       reify_expr Reify.reify_imp k [ True ] [ T ]).
+
+Ltac reify_lemma e :=
+	let T := type of e in reify_lemma_aux T.
+(*
 Ltac reify_lemma e :=
   match type of e with
     | ?T =>
@@ -138,20 +150,25 @@ Ltac reify_lemma e :=
        in
        reify_expr Reify.reify_imp k [ True ] [ T ])
   end.
-
+*)
 Require Import Semantics.
   
 (** Skip **)
-Definition Skip_lemma : lemma typ (expr typ func) (expr typ func).
+Definition skip_lemma : lemma typ (expr typ func) (expr typ func).
 reify_lemma rule_skip.
 Defined.
-Print Skip_lemma.
+Print skip_lemma.
 
-Definition Seq_lemma (c1 c2 : cmd) : lemma typ (expr typ func) (expr typ func).
+Definition skip_lemma2 : lemma typ (expr typ func) (expr typ func).
+reify_lemma rule_skip2.
+Defined.
+Print skip_lemma2.
+
+Definition seq_lemma (c1 c2 : cmd) : lemma typ (expr typ func) (expr typ func).
 Proof.
   reify_lemma (@rule_seq c1 c2).
-Qed.
-Print Seq_lemma.
+Defined.
+Print seq_lemma.
 
 Ltac reify_lemma2 e :=
   match type of e with
@@ -166,17 +183,17 @@ Ltac reify_lemma2 e :=
  (*     reify_expr Reify.reify_imp k [ True ] [ T ])*)
   end.
 
-Definition If_lemma (e : dexpr) (c1 c2 : cmd) : lemma typ (expr typ func) (expr typ func).
+Definition if_lemma (e : dexpr) (c1 c2 : cmd) : lemma typ (expr typ func) (expr typ func).
 Proof.
   reify_lemma (@rule_if e c1 c2).
 Defined.
-Print If_lemma.
+Print if_lemma.
 
 Definition read_lemma (x y f : String.string) : lemma typ (expr typ func) (expr typ func).
 Proof.  
   reify_lemma (@rule_read_fwd x y f).
-  (* Does not work *)
-Admitted.
+Defined.
+Print read_lemma.
 
 Definition write_lemma (x f : String.string) (e : dexpr) : lemma typ (expr typ func) (expr typ func).
 Proof.
@@ -184,11 +201,13 @@ Proof.
 Defined.
 Print write_lemma.
 
+Example test_write x f e : test_lemma (write_lemma x f e). Admitted.
+
 Definition assign_lemma (x : String.string) (e : dexpr) : lemma typ (expr typ func) (expr typ func).
 Proof.
-  reify_lemma2 (@rule_assign_fwd x e).
-  (* Does not work *)
-Admitted.
+  reify_lemma (@rule_assign_fwd x e).
+Defined.
+Print assign_lemma.
 
 Definition pull_exists_lemma : lemma typ (expr typ func) (expr typ func) :=
 {|
@@ -196,134 +215,6 @@ Definition pull_exists_lemma : lemma typ (expr typ func) (expr typ func) :=
  ; premises :=  mkEntails [tySpec, Var 0, mkForall [tySpec, tyVal, mkTriple [App (Var 2) (Var 0), Var 3, Var 4]]] :: nil 
  ; concl := mkEntails [tySpec, Var 0, mkTriple [mkExists [tySasn, tyVal, App (Var 2) (Var 0)], Var 2, Var 3]]
 |}.
-
-
-Definition skip_lemma : lemma typ (expr typ func) (expr typ func) :=
-{| vars := tySpec :: tySasn ::  nil
- ; premises := nil
- ; concl := mkEntails [tySpec, Var 0, mkTriple [Var 1, mkCmd [cskip], Var 1]]
- |}.
- 
-Check test_lemma.
- (* 
-Time Eval compute in (test_lemma skip_lemma).
- *)
-Definition skip_lemma2 : lemma typ (expr typ func) (expr typ func) :=
-{| vars := tySasn ::  nil
- ; premises := nil
- ; concl := mkEntails [tySasn, Var 0, Var 0]
- |}.
- (*
-Eval vm_compute in (test_lemma skip_lemma2).
-*)
-Definition seq_lemma c1 c2 : lemma typ (expr typ func) (expr typ func) :=
-	{| vars := tySpec :: tySasn :: tySasn :: tySasn :: nil;
-	   premises := mkEntails [tySpec, Var 0, mkTriple [Var 1, mkCmd [c1], Var 2]] ::
-                   mkEntails [tySpec, Var 0, mkTriple [Var 2, mkCmd [c2], Var 3]] :: nil;
-       concl := mkEntails [tySpec, Var 0, mkTriple [Var 1, mkCmd [cseq c1 c2], Var 3]]
-    |}.
-
-Example seq_test c1 c2 : test_lemma (seq_lemma c1 c2).
-
-Definition liftVarEq (x : string) (e : expr typ func) := 
-           mkAp [tyVal, tyProp, 
-                 mkAp [tyVal, tyArr tyVal tyProp,
-                       mkConst [tyArr tyVal (tyArr tyVal tyProp), fEq [tyVal]],
-                       App fstack_get (mkString [x])],
-                 e].
-                 
-Definition singleSubst t e x v : expr typ func := 
-            mkSingleSubst [t, e, 
-                           mkString [x], mkConst[tyVal, v]].
-                           
-Definition liftPointsto x f e : expr typ func := 
-	mkAp [tyVal, tyAsn,
-	     mkAp [tyString, tyArr tyVal tyAsn,
-	           mkAp [tyVal, tyArr tyString (tyArr tyVal tyAsn),
-	                 mkConst [tyArr tyVal (tyArr tyString (tyArr tyVal tyAsn)), fPointsto],
-	                 App fstack_get (mkString [x])],
-	           mkConst [tyString, mkString [f]]],
-	    e].
-
-Open Scope string.
-Check @Applicative.ap (Fun stack) (Applicative_Fun _) sval Prop
-	(@Applicative.ap (Fun stack) (Applicative_Fun _) sval (sval -> Prop)
-		(@Applicative.pure (Fun stack) (Applicative_Fun _) (sval -> sval -> Prop) (@eq sval))
-			((fun x s => s x) "a"))
-				((fun x s => s x) "a").
-Definition assign_lemma x e : lemma typ (expr typ func) (expr typ func) :=
-{| vars := tySpec :: tySasn :: (tyArr (tyArr tyString tyVal) tyVal) :: tyString :: nil
- ; premises := nil
- ; concl := mkEntails [tySpec, Var 0, 
-                       mkTriple [Var 1,
-                                 mkCmd [cassign x e], 
-                                 mkExists [tySasn, tyVal, 
-                                         mkAnd [tySasn,
-                                               lembed tyPure tySasn (liftVarEq x (singleSubst tyVal (App fEval (mkExpr [e])) x (Var 0))),
-                                               singleSubst tyAsn (Var 2) x (Var 0)]]]]
-|}.
-
-Example assign_test x e : test_lemma (assign_lemma x e).
-Proof.
-  admit.
-Qed.
-
-Definition write_lemma x f e : lemma typ (expr typ func) (expr typ func) :=
-{| vars := tySpec :: tySasn :: tySasn :: nil
- ; premises := mkEntails [tySasn, Var 1, mkExists [tySasn, tyVal, 
-      											   mkStar [tySasn, 
-      											           Var 3, 
-      											           liftPointsto x f (mkConst [tyVal, Var 0])]]] :: nil
-
- ; concl := mkEntails [tySpec, Var 0, 
-                       mkTriple [Var 1, 
-                                 mkCmd [cwrite x f e], 
-                                 mkStar [tySasn, Var 2, 
-                                         liftPointsto x f (App fEval (mkExpr [e]))]]]
-
-     
- |}.
-
-Example write_test x f e : test_lemma (write_lemma x f e).
-Proof.
-  admit.
-Qed.
-
-Definition read_lemma (x y f : string) : lemma typ (expr typ func) (expr typ func) :=
-{| vars :=  tySpec :: tySasn (*:: tyExpr*) :: nil
- ; premises :=
-     mkEntails [tySasn,
-               Var 1,
-               liftPointsto y f (App fEval (Var 2))] :: nil
- ; concl := 
- mkEntails [tySpec, Var 0,
- mkTriple [Var 1, mkCmd [cread x y f],
- mkExists [tySasn, tyVal,
- mkAnd [tySasn, mkTrue [tySasn],
-     (*   lembed tyPure tySasn (liftVarEq x (App fstack_get (mkString [x])))*) mkTrue [tySasn]
-     (*   singleSubst tyAsn (Var 2) x (Var 0) *)]]]]
-
- 
- 
- (*mkEntails [tySpec,
-                       Var 0,
-                       mkTriple [Var 1, mkCmd [cread x y f],
-                       mkExists [tySasn, tyVal, 
-                                 mkAnd [tySasn, 
-                                        lembed tyPure tySasn
-                                           (*    (liftVarEq x (singleSubst tyVal (App fEval (Var 3)) x (Var 0)))*)
-(           mkAp [tyVal, tyProp, 
-                 mkAp [tyVal, tyArr tyVal tyProp,
-                       mkConst [tyArr tyVal (tyArr tyVal tyProp), fEq [tyVal]],
-                       App fstack_get (mkString [x])],
-                 App fstack_get (mkString [x])]),
-                                        singleSubst tyAsn (Var 2) x (Var 0)]]]]*)
- |}.
-
-Example read_test x y f : test_lemma (read_lemma x y f).
-Proof. cbv.
-   admit.
-Qed.
 
 Definition fieldLookupTac : stac typ (expr typ func) subst :=
 	fun tus tvs s lst e =>
@@ -340,82 +231,6 @@ Definition fieldLookupTac : stac typ (expr typ func) subst :=
 		    end
 		  | _ => Fail
 		end.
-
-Definition alloc_lemma x C : lemma typ (expr typ func) (expr typ func) :=
-  {|
-     vars := tySpec :: tySasn :: tyProg :: tyFields :: nil;
-     premises := mkEntails [tySpec, Var 0, mkProgEq [Var 2]] :: 
-                 mkFieldLookup [Var 2, mkString [C], Var 3] :: nil;
-     concl := mkEntails [tySpec, Var 0,
-                         mkTriple [Var 1, mkCmd [calloc x C], 
-                                   mkExists[tySasn, tyVal,
-                                           mkSetFold [mkString [x], Var 4, 
-                                                      mkSingleSubst[tyAsn, Var 2, mkString [x], mkConst[tyVal, Var 0]]]]]]
-  |}.
-
-Example alloc_test x C : test_lemma (alloc_lemma x C).
-Proof.
-	admit.
-Qed.
-
-Definition dcall_lemma x (y : var) m es : lemma typ (expr typ func) (expr typ func) :=
-  {|
-     vars := tySpec :: tySasn :: tyString :: tyVarList :: tyString :: tySasn :: tySasn :: tySasn :: nil;
-     premises := mkEntails [tySasn, Var 1, lembed tyPure tySasn 
-                                                  (mkAp [tyVal, tyProp, 
-                                                   mkAp [tyString, tyArr tyVal tyProp,
-                                                         mkConst [tyArr tyString (tyArr tyVal tyProp), fTypeOf],
-                                                         mkConst [tyString, Var 2]],
-                                                   (App fstack_get (mkString [y]))])] :: 
-                mkEntails [tySpec, Var 0, mkMethodSpec [Var 2, mkString [m], Var 3, Var 4, Var 5, Var 6]] ::
-                mkEq [tyNat, mkLengthVarList [Var 3], mkExprList [(E_var y)::es]] ::
-                mkEntails [tyAsn, Var 1, mkStar [tySasn, mkSubst [tyAsn, Var 5, mkSubstList [Var 3, mkExprList [(E_var y)::es]]], Var 7]] ::
-                nil ;
-     concl := mkEntails [tySpec, Var 0, 
-                         mkTriple [Var 1, mkCmd [cdcall x y m es], 
-                                   mkExists [tySasn, tyVal, 
-                                           mkAnd [tySasn, lembed tyPure tySasn 
-                                                  (mkAp [tyVal, tyProp, 
-                                                   mkAp [tyString, tyArr tyVal tyProp,
-                                                         mkConst [tyArr tyString (tyArr tyVal tyProp), fTypeOf],
-                                                         mkConst [tyString, Var 3]],
-                                                   mkSingleSubst [tyVal, App fstack_get (mkString [y]), mkString [x], mkConst[tyVal, Var 0]]]),
-                                           mkStar [tySasn,
-                                           mkSubst [tyAsn, Var 7, 
-                                                    mkSubstList [mkConsVarList[Var 5, Var 4], 
-                                                                mkConsExprList [App fstack_get (mkString [x]), 
-                                                                                mkConsExprList [mkSingleSubst [tyVal, App fstack_get (mkString [y]), mkString [x], mkConst [tyVal, Var 0]],
-                                                                                                mkSubstExprList [es, mkString [x], mkConst[tyVal, Var 0]]]]]],
-                                           mkSingleSubst[tyAsn, Var 8, mkString [x], mkConst[tyVal, Var 0]]]]]]]
-  |}.
-
-Example dcall_test x y m es : test_lemma (dcall_lemma x y m es).
-Proof.
-   admit.
-Qed.
-
-Definition scall_lemma x (C : class) m es : lemma typ (expr typ func) (expr typ func) :=
-  {|
-     vars := tySpec :: tySasn :: tyVarList :: tyString :: tySasn :: tySasn :: tySasn :: nil;
-     premises := mkEntails [tySpec, Var 0, mkMethodSpec [mkString [C], mkString [m], Var 2, Var 3, Var 4, Var 5]] ::
-                 mkEq [tyNat, mkLengthVarList [Var 3], mkExprList [es]] ::
-                 mkEntails [tyAsn, Var 1, mkStar [tySasn, mkSubst [tyAsn, Var 4, mkSubstList [Var 2, mkExprList [es]]], Var 6]] ::
-                 nil ;
-     concl := mkEntails [tySpec, Var 0, 
-                         mkTriple [Var 1, mkCmd [cscall x C m es], 
-                                   mkExists [tySasn, tyVal, 
-                                           mkStar [tySasn,
-                                           mkSubst [tyAsn, Var 6, 
-                                                    mkSubstList [mkConsVarList[Var 5, Var 4], 
-                                                                mkConsExprList [App fstack_get (mkString [x]), 
-                                                                                mkSubstExprList [es, mkString [x], mkConst[tyVal, Var 0]]]]],
-                                           mkSingleSubst[tyAsn, Var 7, mkString [x], mkConst[tyVal, Var 0]]]]]]
-  |}.
-
-Example scall_test x C m es : test_lemma (scall_lemma x C m es).
-Proof.
-   admit.
-Qed.
 
 Let EAPPLY lem tac :=
   @EAPPLY typ (expr typ func) subst _ _ ExprLift.vars_to_uvars
@@ -434,17 +249,23 @@ Let EAPPLY lem tac :=
            (@ExprSubst.instantiate typ func) SS SU
            lem (apply_to_all tac).
 
+Require Import MirrorCharge.Java.Subst.
+Check @INSTANTIATE.
+Let INSTANTIATE := 
+	@INSTANTIATE typ (expr typ func) subst (@ExprSubst.instantiate typ func) SS.
+
 Definition solve_entailment :=
-  REPEAT 5 (APPLY pull_exists_lemma
-  (THEN (SIMPLIFY (fun _ _ _ => beta_all simplify nil nil))
-       stac_cancel)).
+  THEN (TRY (APPLY pull_exists_lemma (@IDTAC _ _ _)))
+       (THEN INSTANTIATE (THEN
+             (SIMPLIFY (fun _ _ _ => beta_all simplify nil nil))
+                        stac_cancel)).
 
 Fixpoint tripleE (c : cmd) : stac typ (expr typ func) subst :=
 	match c with
 	    | cskip => EAPPLY skip_lemma solve_entailment
 		| cseq c1 c2 => EAPPLY (seq_lemma c1 c2) (FIRST (tripleE c1::tripleE c2::nil))
 		| cassign x e => EAPPLY (assign_lemma x e) solve_entailment
-		| cread x y f => EAPPLY (read_lemma x y f) (@IDTAC _ _ _)
+		| cread x y f => EAPPLY (read_lemma x y f) solve_entailment
 		| cwrite x f e => EAPPLY (write_lemma x f e) solve_entailment
 		| _ => @IDTAC _ _ _
 	end.
@@ -456,17 +277,33 @@ Definition symE : stac typ (expr typ func) subst :=
 			  (tripleE c) tus tvs s lst e 
 			| _ => Fail
 		end.  
+		
+Require Import Java.Semantics.OperationalSemantics.
+Require Import Java.Logic.SpecLogic.
+Require Import Java.Logic.AssertionLogic.
+
+Require Import Charge.Logics.ILogic.
 
 Definition testSkip :=
   let vars := tySpec :: tySasn :: nil in
   let goal :=
       mkEntails [tySpec, Var 0,
-                 mkTriple [Var 1, mkCmd [cseq cskip (cseq cskip cskip)], Var 1]]
+                 mkTriple [Var 1, mkCmd [cskip], Var 1]]
   in
   @symE nil vars (SubstI.empty (expr :=expr typ func)) nil goal.
- 
+  
 Time Eval vm_compute in testSkip.
 
+Definition mkPointsto x f e : expr typ func :=
+(mkAp [tyVal, tyAsn, 
+                      mkAp [tyString, tyArr tyVal tyAsn,
+                            mkAp [tyVal, tyArr tyString (tyArr tyVal tyAsn),
+                                  mkConst [tyArr tyVal (tyArr tyString (tyArr tyVal tyAsn)), fPointsto],
+                                  App fStackGet (mkString [x])],
+                            mkConst [tyString, mkString [f]]],
+                      e]).
+
+Require Import String.
 Open Scope string.
 
 Definition test_read :=
@@ -474,29 +311,81 @@ Definition test_read :=
   let vars := nil in
   let goal :=
   	mkEntails [tySpec, mkTrue [tySpec], 
-  	           mkTriple [(*liftPointsto "o" "f" (App fEval (Var 1))*) mkTrue [tySasn],
+  	           mkTriple [ mkPointsto "o" "f" (mkConst [tyVal, mkVal [vint 3]]),
   	                     mkCmd [cread "x" "o" "f"],
   	                     (UVar 0)]]
   in
-  let tac := symE in
-  @tac uvars vars (SubstI.empty (expr :=expr typ func)) nil goal.
-
+  @symE uvars vars (SubstI.empty (expr :=expr typ func)) nil goal.
 Time Eval vm_compute  in test_read.
 
+Require Import Charge.Logics.BILogic.
+
+Definition testWrite :=
+  let uvars := tySasn :: nil in
+  let vars := nil in
+  let goal :=
+  	mkEntails [tySpec, mkTrue [tySpec], 
+  	           mkTriple [mkStar [tySasn, mkEmp [tySasn], mkPointsto "o" "f" (mkConst [tyVal, mkVal [vint 3]])],
+  	                     mkCmd [cwrite "o" "f" (E_val (vint 0))],
+  	                     (UVar 0)]]
+  in
+  @symE uvars vars (SubstI.empty (expr :=expr typ func)) nil goal.
+Time Eval vm_compute  in testWrite.
+Print write_lemma.
+
+Opaque the_canceller.
+Goal (exists x, x = testWrite).
+cbv.
+Transparent the_canceller.
+Check @the_canceller.
+match goal with | |- context [the_canceller ?a ?b ?c ?d ?e] => 
+pose (the_canceller a b c d e); pose a; pose b; pose c; pose d
+end.
+Check exprD'.
+pose (exprD' l l0 e0 tySasn).
+simpl in r.
+red in r.
+simpl in r.
+unfold Open_App in r.
+simpl in r.
+unfold Open_Inj in r.
+simpl in r.
+unfold Rcast_val in r.
+simpl in r. 
+unfold Rcast in r; simpl in r.
+
+pose (exprD' l l0 e tySasn).
+simpl in r0.
+red in r0.
+simpl in r0.
+unfold Open_App in r0.
+simpl in r0.
+unfold Open_Inj in r0.
+simpl in r0.
+unfold Rcast_val in r0.
+simpl in r0. 
+unfold Rcast in r; simpl in r0.
+
+Eval cbv beta iota zeta delta [exprD' Expr_expr] in (exprD' nil nil e (tySasn)).
+cbv in s.
+
+Check stac_cancel.
+Print stac.
+simpl.
 Definition testSwap :=
   let uvars := nil in
   let vars := tyExpr :: tyExpr :: nil in
   let goal := mkEntails [tySpec, mkTrue [tySpec],
   	                     mkTriple [mkStar [tySasn,
-  		                                   liftPointsto "o" "f1" (App fEval (Var 0)),
-	  	                                   liftPointsto "o" "f2" (App fEval (Var 1))],                                           	                      
+  		                                   mkPointsto "o" "f1" (App fEval (Var 0)),
+	  	                                   mkPointsto "o" "f2" (App fEval (Var 1))],                                           	                      
   	                               mkCmd [cseq (cread "x1" "o" "f1")
   	                                      (cseq (cread "x2" "o" "f2")
   	                                      (cseq (cwrite "o" "f1" (E_var "x2"))
   	                                            (cwrite "o" "f2" (E_var "x1"))))], 
 			                       mkStar [tySasn,
-			                               liftPointsto "o" "f1" (App fEval (Var 1)),
-			                               liftPointsto "o" "f2" (App fEval (Var 0))]]]                                     
+			                               mkPointsto "o" "f1" (App fEval (Var 1)),
+			                               mkPointsto "o" "f2" (App fEval (Var 0))]]]                                     
   in
   let tac := symE in
   @tac uvars vars (SubstI.empty (expr :=expr typ func)) nil goal.
